Leanegraph/core/Theorems.lean
@@ -10,29 +10,159 @@ variable {D : Type _} [DecidableEq D] [Inhabited D]
 
 namespace Naive
 
-theorem pushPreservesAlwaysInvariants [Analysis α D] (eg : EGraph α D)
+theorem lookupAfterUnionSome [Analysis α D] (eg : EGraph α D) (en : ENode α) (id₁ id₂ id : EClassId)
+    (hcsome : eg.hcons.lookup en = some id):
+      (union eg id₁ id₂).fst.hcons.lookup en = some id := by
+  simp[union]
+  split
+  case isTrue h =>
+    simp[hcsome]
+  case isFalse h =>
+    simp[hcsome]
+
+theorem lookupBeforeUnionSome [Analysis α D] (eg : EGraph α D) (en : ENode α) (id₁ id₂ id : EClassId)
+    (hcsome : (union eg id₁ id₂).fst.hcons.lookup en = some id)
+    : eg.hcons.lookup en = some id
+    := by
+  simp[union] at hcsome
+  split at hcsome
+  case isTrue h =>
+    simpa using hcsome
+  case isFalse h =>
+    simpa using hcsome
+
+theorem unionDoesntChangeHCLookupSome [Analysis α D] (eg : EGraph α D) (en : ENode α) (id₁ id₂ id : EClassId) :
+    eg.hcons.lookup en = some id ↔  (union eg id₁ id₂).fst.hcons.lookup en = some id := by
+  apply Iff.intro
+  exact lookupAfterUnionSome eg en id₁ id₂ id
+  exact lookupBeforeUnionSome eg en id₁ id₂ id
+
+omit [DecidableEq D] [Inhabited D] in
+theorem canonicaliseIdem [Analysis α D] (eg : EGraph α D) (en : ENode α) (h : eg.uf.isCanon) :
+    (canonicalise eg en) = canonicalise eg (canonicalise eg en) := by
+  simp[canonicalise]
+  intro ecid mem
+  simp[lookupCanonicalEClassId]
+  have hidemp := UF.findIdempotent eg.uf h ecid
+  exact hidemp.symm
+
+omit [DecidableEq D] in
+theorem pushEnEqPushCanonEn [Analysis α D] (eg : EGraph α D) (en : ENode α) (h : eg.alwaysInvariants) :
+    push eg en = push eg (canonicalise eg en) := by
+  unfold push
+  simp only
+  have pushpush := canonicaliseIdem eg en h.1.2.1
+  rw[←pushpush] -- interesting that rw[pushpush] did not work despite them should be equal?
+
+omit [DecidableEq α] [Hashable α] [DecidableEq D] [Inhabited D] in
+theorem updateParents_lookup (ecmap : ListMap EClassId (EClass α D)) (en : ENode α) (id k : EClassId) :
+    (updateParents ecmap en id).lookup k =
+      if k ∈ en.args then
+        (ecmap.lookup k).map (updateEClassParents en id)
+      else
+        ecmap.lookup k
+    := by
+  unfold updateParents
+  simp[ListMap.lookup, ListMap.map]
+  induction ecmap.val with
+  | nil => simp
+  | cons x xs ih =>
+    rcases x with ⟨k', cls⟩
+    simp[List.map, List.lookup]
+    by_cases eq : k = k'
+    ·
+      simp[eq]
+      -- already equal though, just some (if a else b) and if (some a) else (some b)
+      -- cant find a theorem
+      by_cases hm : k' ∈ en.args
+      <;> simp[hm]
+    ·
+      have hnq : ¬(k == k') := by simp[eq]
+      simp[hnq, ih]
+
+
+
+theorem lookupAfterPushECMap [Analysis α D] (eg : EGraph α D) (en : ENode α) (id : EClassId)
+    (h : id = eg.uf.push.snd) :
+    eg.ecmap.lookup id = (push eg en).fst.ecmap.lookup id := by
+  simp[push]
+  split
+  case h_1 oid ecid hSome =>
+    simp
+  case h_2 oid hNone =>
+    simp[insertECMap]
+    simp[ListMap.insert]
+
+    simp[uniqueInsert]
+
+    simp[h]
+
+    simp[ListMap.lookup]
+
+
+
+
+    sorry
+
+omit [DecidableEq D] in
+theorem lookupAfterPushECMapNE [Analysis α D] (eg : EGraph α D) (en : ENode α) (id : EClassId)
+    (h : ¬id = eg.uf.push.snd) (hnm : id ∉ (canonicalise eg en).args) :
+    eg.ecmap.lookup id = (push eg en).fst.ecmap.lookup id := by
+  unfold push
+  simp
+  split
+  case h_1 oid ecid hSome =>
+    rfl
+  case h_2 oid hNone =>
+    unfold insertECMap
+    simp
+    /-
+    have aa := ListMap.lookupAfterInsertNE eg.ecmap eg.uf.push.snd (EClass.fromNode (canonicalise eg en)
+          (Analysis.make (canonicalise eg en)
+            (List.map (fun id => ((ecmapLookup eg id).getD EClass.empty).data) (canonicalise eg en).args))) id h
+    -/
+    simp[ListMap.lookupAfterInsertNE _ _ _ _ h] -- thanks lean for the inference
+    rw[updateParents_lookup]
+    simp[hnm]
+
+/-
+  Section 1: AlwaysInvariants
+-/
+
+/-
+  Section 1.1: Push Operation Preserves EGraph alwaysInvariants
+  - UF: isValid, isCanon, hasRep, isComplete, uniqueKeys
+  - The other EGraph ones, TODO: name them later because I'll keep adding to them
+-/
+omit [DecidableEq D] in
+theorem EGraph.pushPreservesIsValid [Analysis α D] (eg : EGraph α D)
   (h : eg.alwaysInvariants) (en : ENode α) :
-    (push eg en).1.alwaysInvariants := by
-  unfold EGraph.alwaysInvariants
+    (push eg en).fst.uf.isValid := by
   unfold EGraph.alwaysInvariants at h
-  rcases h with ⟨hUfWf, hDv, hAv, hHcEm⟩
+  rcases h with ⟨hUfWf, hDv, hAv, hHcEm, hhcv, hepv⟩
   rcases hUfWf with ⟨hUfv, hUfc, hR, hCmp, hU⟩
-  constructor
-  constructor
-  · -- isValid
+  -- isValid
     -- show that pushing does not change the validity of the unionfind
     -- do we not have this already?
-    have isValid := UF.pushPreservesValid _ hUfv
+  have isValid := UF.pushPreservesValid _ hUfv
 
-    unfold push
-    dsimp
-    split
-    ·
-      exact hUfv
-    case h_2 optEid noneLookup =>
-      simp[isValid]
-  constructor
-  · -- isCanon
+  unfold push
+  dsimp
+  split
+  ·
+    exact hUfv
+  case h_2 optEid noneLookup =>
+    simp[isValid]
+
+omit [DecidableEq D] in
+theorem EGraph.pushPreservesIsCanon [Analysis α D] (eg : EGraph α D)
+  (h : eg.alwaysInvariants) (en : ENode α) :
+    (push eg en).fst.uf.isCanon := by
+    have hinvar := h
+    unfold EGraph.alwaysInvariants at h
+    rcases h with ⟨hUfWf, hDv, hAv, hHcEm, hhcv, hepv⟩
+    rcases hUfWf with ⟨hUfv, hUfc, hR, hCmp, hU⟩
+    -- isCanon
     -- show that pushing does not change the canonicity of the unionfind
     have isCanon := UF.pushPreservesCanon _ hUfc hUfv
     unfold push
@@ -42,68 +172,496 @@ theorem pushPreservesAlwaysInvariants [Analysis α D] (eg : EGraph α D)
       simp[hUfc]
     case h_2 eid lookupNone =>
       exact isCanon
+
+omit [DecidableEq D] in
+theorem EGraph.pushPreservesHasRep [Analysis α D] (eg : EGraph α D)
+  (h : eg.alwaysInvariants) (en : ENode α) :
+    (push eg en).fst.uf.hasRep := by
+  have hinvar := h
+  unfold EGraph.alwaysInvariants at h
+  rcases h with ⟨hUfWf, hDv, hAv, hHcEm, hhcv, hepv⟩
+  rcases hUfWf with ⟨hUfv, hUfc, hR, hCmp, hU⟩
+  have hasRep := UF.pushPreservesReps eg.uf hR
+  unfold push
+  dsimp
+  split
+  case h_1 ecId id lookupSome =>
+    simp[hR]
+  case h_2 eid lookupNone =>
+    exact hasRep
+
+omit [DecidableEq D] in
+theorem EGraph.pushPreservesIsComplete [Analysis α D] (eg : EGraph α D)
+  (h : eg.alwaysInvariants) (en : ENode α) :
+    (push eg en).fst.uf.isComplete := by
+  have hinvar := h
+  unfold EGraph.alwaysInvariants at h
+  rcases h with ⟨hUfWf, hDv, hAv, hHcEm, hhcv, hepv⟩
+  rcases hUfWf with ⟨hUfv, hUfc, hR, hCmp, hU⟩
+  have hComp := UF.pushPreservesComplete eg.uf hinvar.1
+  unfold push
+  dsimp
+  split
+  case h_1 ecId id lookupSome =>
+    simp[hCmp]
+  case h_2 eid lookupNone =>
+    simp[hComp]
+
+
+omit [DecidableEq D] in
+theorem EGraph.pushPreservesUniqueKeys [Analysis α D] (eg : EGraph α D)
+  (h : eg.alwaysInvariants) (en : ENode α) :
+    (push eg en).fst.uf.uniqueKeys := by
+  have hinvar := h
+  unfold EGraph.alwaysInvariants at h
+  rcases h with ⟨hUfWf, hDv, hAv, hHcEm, hhcv, hepv⟩
+  rcases hUfWf with ⟨hUfv, hUfc, hR, hCmp, hU⟩
+  have hPuk := UF.pushPreservesUniqueKeys eg.uf hinvar.1
+  unfold push
+  dsimp
+  split
+  case h_1 ecId id lookupSome =>
+    simp[hU]
+  case h_2 eid lookupNone =>
+    simp[hPuk]
+
+omit [DecidableEq D] in
+theorem EGraph.pushPreservesWellFormed [Analysis α D] (eg : EGraph α D)
+  (h : eg.alwaysInvariants) (en : ENode α) :
+    (push eg en).fst.uf.wellFormed :=
+  ⟨
+    eg.pushPreservesIsValid h en,
+    eg.pushPreservesIsCanon h en,
+    eg.pushPreservesHasRep h en,
+    eg.pushPreservesIsComplete h en,
+    eg.pushPreservesUniqueKeys h en
+  ⟩
+
+omit [DecidableEq D] in
+theorem EGraph.pushPreservesDirty [Analysis α D] (eg : EGraph α D)
+  (h : eg.alwaysInvariants) (en : ENode α) :
+    (push eg en).fst.dirtyValid := by
+  have hinvar := h
+  unfold EGraph.alwaysInvariants at h
+  rcases h with ⟨hUfWf, hDv, hAv, hHcEm, hhcv, hepv⟩
+  rcases hUfWf with ⟨hUfv, hUfc, hR, hCmp, hU⟩
+-- dirtyValid
+  unfold push
+  dsimp
+  split
+  case h_1 opeid id lookupSome =>
+    exact hDv
+  case h_2 oid lookupNone =>
+    simp only
+    unfold EGraph.dirtyValid
+    intro id hmem
+    dsimp at *
+    unfold UF.isValidID
+    have hmem' := List.mem_cons.mp hmem
+    rcases hmem' with hnew | hold
+    ·
+      simp[hnew, UF.push, UF.size]
+    ·
+      simp[UF.push, UF.size]
+      simp[UF.push, UF.size] at hmem
+      rcases hmem with rfl | hold
+      ·
+        simp
+      ·
+        have hid := hDv id hold
+        simp[UF.isValidID] at hid
+        simp[UF.size] at hid
+        have hpo : id < List.length eg.uf + 1 := Nat.lt_trans hid (Nat.lt_add_one _)
+        exact hpo
+
+omit [DecidableEq D] in
+theorem EGraph.pushPreservesAldrt [Analysis α D] (eg : EGraph α D)
+  (h : eg.alwaysInvariants) (en : ENode α) :
+    (push eg en).fst.aldrtValid := by
+  have hinvar := h
+  unfold EGraph.alwaysInvariants at h
+  rcases h with ⟨hUfWf, hDv, hAv, hHcEm, hhcv, hepv⟩
+  rcases hUfWf with ⟨hUfv, hUfc, hR, hCmp, hU⟩
+  unfold push
+  dsimp only
+  split
+  case h_1 oeid id lookupSome =>
+    exact hAv
+  case h_2 oeid lookupNone =>
+    simp only
+    unfold EGraph.aldrtValid
+    intro id hmem
+    dsimp at *
+    unfold UF.isValidID
+    have hmem' := List.mem_cons.mp hmem
+    rcases hmem' with hnew | hold
+    ·
+      simp[hnew, UF.push, UF.size]
+    ·
+      simp[UF.push, UF.size]
+      simp[UF.push, UF.size] at hmem
+      rcases hmem with rfl | hold
+      ·
+        simp
+      ·
+        have hid := hAv id hold
+        simp[UF.isValidID, UF.size] at hid
+        exact Nat.lt_trans hid (Nat.lt_add_one _)
+
+omit [DecidableEq D] in
+theorem EGraph.pushPreservesHConsValidity [Analysis α D] (eg : EGraph α D)
+  (h : eg.alwaysInvariants) (en : ENode α) :
+    (push eg en).fst.hconsValidity := by
+  have hinvar := h
+  unfold EGraph.alwaysInvariants at h
+  rcases h with ⟨hUfWf, hDv, hAv, hHcEm, hhcv, hepv⟩
+  rcases hUfWf with ⟨hUfv, hUfc, hR, hCmp, hU⟩
+  unfold push
+  dsimp only
+  -- simp[EGraph.hconsValidity] at *
+  intro en' id' hex
+  split
+  case h_1 oid id hSome =>
+    simp[hSome] at hex
+    simp only
+    unfold EGraph.hconsValidity at hhcv
+    exact hhcv en' id' hex
+  case h_2 oid hNone =>
+    simp[hNone] at hex
+    simp
+    by_cases heq : en' = (canonicalise eg en)
+    ·
+      subst heq
+      have lai := ListMap.lookupAfterInsert eg.hcons (canonicalise eg en) eg.uf.push.snd
+      unfold insertHCons at hex
+      rw[lai] at hex
+      rw[hex] at lai
+      injection hex with eq
+      rw[←eq]
+      have ans := UF.pushReturnsValidID eg.uf
+      exact ans
+    ·
+      have lain := ListMap.lookupAfterInsertNE eg.hcons (canonicalise eg en) eg.uf.push.snd en' heq
+      simp[insertHCons] at hex
+      rw[lain] at hex
+      -- unfold EGraph.hconsValidity at hhcv
+      exact UF.pushPreservesValidID eg.uf id' (hhcv en' id' hex)
+  /-
+    -- en' doesn't exist in hashcons, id' is therefore nonexistent
+    -- until we push it in that is
+    simp[hNone] at hex
+    simp only
+    unfold EGraph.hconsValidity at hhcv
+    unfold insertHCons at hex -- need a lemma saying lookupAfterInsert returns inserted
+    have hex' := eg.hcons.lookupAfterInsert (canonicalise eg en) id'
+    -- rw[hex'] at hex
+    by_cases heq : en' = (canonicalise eg en)
+    case pos =>
+      subst heq
+      have ans := hhcv (canonicalise eg en) id'
+      have fnd := ListMap.lookupAfterInsert eg.hcons (canonicalise eg en) eg.uf.push.snd
+      simp[fnd] at hex
+      rw[hex] at fnd
+      subst hex
+
+
+      sorry
+    case neg =>
+
+      sorry
+  -/
+
+omit [DecidableEq D] [Inhabited D] in
+theorem updateParentsByCases [Analysis α D] (eg : EGraph α D)
+    (en : ENode α) (new_id : EClassId) (id : EClassId) (new_cls : EClass α D) :
+    (updateParents eg.ecmap en new_id).lookup id = some new_cls →
+    ∃ old_cls, eg.ecmap.lookup id = some old_cls ∧
+      ∀ p, p ∈ new_cls.parents → p ∈ old_cls.parents ∨ p = (en, new_id) := by
+  intro hlookup
+  rw[updateParents_lookup] at hlookup
+  by_cases harg : id ∈ en.args
+  case pos =>
+    simp[harg] at hlookup
+    rcases hlookup with ⟨oldCls, hOld, hEq⟩
+    exists oldCls
+    constructor
+    exact hOld
+    intro p hp
+    rw [← hEq] at hp
+    simp [updateEClassParents] at hp
+    rcases hp
+    case right.inl hp =>
+      unfold updateEClassParents at hEq
+      rcases hEq with ⟨aaaaa⟩
+      right
+      exact hp
+    ·
+      left
+      assumption
+  ·
+    simp[harg] at hlookup
+    exists new_cls
+    constructor
+    exact hlookup
+    intro p hp
+    left
+    exact hp
+
+omit [DecidableEq D] in
+theorem EGraph.pushPreservesECMapParentsValid [Analysis α D] (eg : EGraph α D)
+  (h : eg.alwaysInvariants) (en : ENode α) :
+    (push eg en).fst.ecmapParentsValid := by
+  have hinvar := h
+  unfold EGraph.alwaysInvariants at h
+  rcases h with ⟨hUfWf, hDv, hAv, hHcEm, hhcv, hepv⟩
+  rcases hUfWf with ⟨hUfv, hUfc, hR, hCmp, hU⟩
+  intro id cls hlookup p pmem
+  unfold push
+  dsimp
+  -- have aa := updateParentsByCases eg en (push eg en).snd id cls
+  -- have bb := updateParentsByCases eg (canonicalise eg en) eg.uf.push.snd id cls
+  -- have cc := updateParents_lookup eg.ecmap (canonicalise eg en) eg.uf.push.snd id
+  -- simp[push] at hlookup
+
+  split
+  case h_1 oid eid heq =>
+    simp
+    simp[push, heq] at hlookup pmem
+    exact hepv id cls hlookup p pmem
+  case h_2 eid hnq =>
+    simp
+    simp[push, hnq, insertECMap] at hlookup pmem
+    by_cases hideq : id = eg.uf.push.snd
+    ·
+      rw[hideq] at hlookup
+      rw[ListMap.lookupAfterInsert] at hlookup
+      rw[Option.some.injEq] at hlookup
+      rw[←hlookup] at pmem
+      unfold EClass.fromNode at pmem
+      simp at pmem
+    ·
+      simp[ListMap.lookupAfterInsertNE _ _ _ _ hideq] at hlookup
+      have upc := updateParentsByCases eg (canonicalise eg en) eg.uf.push.snd id cls hlookup
+      rcases upc with ⟨old, hold, hpc⟩
+      have pc := hpc p pmem
+      cases pc
+      case neg.inl h =>
+        -- case p was from the old parents
+        have oldhepv := hepv id old hold p h
+        exact UF.pushPreservesValidID eg.uf p.snd oldhepv
+      case neg.inr h =>
+        -- case p was a new node (did not exist in parents)
+        have hp2 : p.snd = eg.uf.push.snd := by
+          rw[h]
+        rw[hp2]
+        exact UF.pushReturnsValidID eg.uf
+
+
+  -- do i split here?
+  /-
+  unfold ecmapParentsValid
+  intro id cls lookupSome p pmem
+  unfold push
+  dsimp
+  split
+  case h_1 oid ecid hSome =>
+    simp
+    unfold hcLookup at hSome
+    /-
+      If you unfold push at lookupSome, you see that node is canonicalised before pushing
+      and we see that push also adds it to the hcons
+      Therefor (push eg en) adds a canonicalised en (call it c_en) to both hcons and ecmap
+      So then we can see that ecmap.lookup returns a class
+      and hSome returns an ecid
+      so canonical rep of ecls is ecid?
+      But that's not what we want
+
+      Try again
+
+      Is this supposed to be an induction proof? no
+
+      idea 1: show that push eg en is equal to push eg (canonicalise eg en)
+      then we can rewrite something
+      i had this idea in a dream but now i forgot what exactly it was
+      also need to show idempotence of canonicalise, lets start with that
+      ok
+
+      where was i
+
+      wait do i even need to do this
+
+    -/
+
+    have aa := hhcv p.1 p.snd
+    have bb := hepv ecid cls
+    sorry
+  case h_2 oid hNone =>
+    simp
+
+    sorry
+  -/
+  /-
+    idea 2: push doesn't touch parents at all
+    try and get that idea through
+    idea 2 sucks, it does touch parents
+    tip: re-read definitions if you forgot
+  -/
+  /-
+    idea 3: split on something else
+    something like
+    id_exists_in_parents_already_and_is_updated
+    vs
+    id_does_not_exist_and_need_to_be_added
+    but cannot split on p ∈ cls.parents
+    so i guess helper lemma?
+  -/
+
+
+theorem EGraph.unionPreservesECMapParentsValid [Analysis α D] (eg : EGraph α D)
+  (h : eg.alwaysInvariants) (id₁ id₂ : EClassId) :
+    -- (h₁ : eg.uf.isValidID id₁) (h₂ : eg.uf.isValidID id₂) : -- why are h₁ h₂ unused? did i make life difficult?
+    (union eg id₁ id₂).fst.ecmapParentsValid := by
+  have hinvar := h
+  unfold EGraph.alwaysInvariants at h
+  rcases h with ⟨hUfWf, hDv, hAv, hHcEm, hhcv, hepv⟩
+  rcases hUfWf with ⟨hUfv, hUfc, hR, hCmp, hU⟩
+  intro id cls hlookup p pmem
+
+  unfold union
+  dsimp
+
+  split
+  case isTrue heq =>
+    -- no union done
+    simp only
+    simp[union, heq] at hlookup
+    simp[UF.isValid] at hUfv
+    simp[ecmapParentsValid] at hepv
+
+    rcases p with ⟨a, b⟩
+    simp[hepv id cls hlookup a b pmem]
+  case isFalse hnq =>
+    simp only
+    simp[union, hnq] at hlookup
+    simp[UF.union, lookupCanonicalEClassId]
+    rw[UF.findIdempotent eg.uf hUfc id₁, UF.findIdempotent eg.uf hUfc id₂]
+    rw[←lookupCanonicalEClassId, ←lookupCanonicalEClassId]
+    simp[hnq]
+
+    simp[UF.isValidID, UF.size]
+
+    -- ⊢ p.snd < List.length eg.uf, so just need to show p.snd is valid
+    -- have test : eg.uf.isValidID p.snd := by sorry
+
+    rw[ecmapParentsValid] at hepv
+    /-
+    hepv : ∀ (id : EClassId) (cls : EClass α D),
+              eg.ecmap.lookup id = some cls →
+              ∀ (p : ENode α × EClassId), p ∈ cls.parents →
+              eg.uf.isValidID p.snd
+
+    Need: eg.ecmap.lookup id = some cls
+    So simplify hlookup as usual
+    -/
+
+    /-
+    wish this was possible
+    let cid₂ := lookupCanonicalEClassId eg id₂
+    let cid₁ := lookupCanonicalEClassId eg id₁
+
+    rw[←cid₂, ←cid₁] at hlookup
+    -/
+    -- this was longer than i expected
+
+    by_cases l₂ : id = (lookupCanonicalEClassId eg id₂)
+    ·
+      simp[l₂, ListMap.lookupAfterInsert] at hlookup
+      simp[EClass.empty] at hlookup
+      simp[←hlookup] at pmem
+      -- contr.
+    ·
+      rw[ListMap.lookupAfterInsertNE _ _ _ _ l₂] at hlookup
+      rw[lookupCanonicalEClassId, lookupCanonicalEClassId] at hlookup
+      rw[unionOfCanonsReturnsFirstArg eg.uf id₁ id₂ hUfc] at hlookup
+
+      by_cases hroot : id = lookupCanonicalEClassId eg id₁
+      case pos =>
+        simp[hroot, lookupCanonicalEClassId] at hlookup
+
+        simp[ListMap.lookupAfterInsert] at hlookup
+
+        simp[EClass.merge] at hlookup
+        rw[←hlookup] at pmem
+        simp[List.mem_append] at pmem
+        cases pmem
+        case inl from1 =>
+          have lookup1 : eg.ecmap.lookup (eg.uf.find id₁) = some ((eg.ecmap.lookup (eg.uf.find id₁)).getD EClass.empty) := by
+            simp[Option.getD]
+            cases h : eg.ecmap.lookup (eg.uf.find id₁) with
+            | none =>
+              simp[h] at from1
+              simp[EClass.empty] at from1
+            | some x =>
+              simp
+          exact hepv (eg.uf.find id₁) _ lookup1 p from1
+        case inr from2 =>
+          have lookup2 : eg.ecmap.lookup (eg.uf.find id₂) = some ((eg.ecmap.lookup (eg.uf.find id₂)).getD EClass.empty) := by
+            simp[Option.getD]
+            cases h : eg.ecmap.lookup (eg.uf.find id₂) with
+            | none =>
+              simp[h] at *
+              simp[EClass.empty] at from2
+            | some x =>
+              simp
+          exact hepv _ _ lookup2 _ from2
+      case neg =>
+        rw[←lookupCanonicalEClassId] at hlookup
+        rw[ListMap.lookupAfterInsertNE _ _ _ _ hroot] at hlookup
+        exact hepv _ _ hlookup p pmem
+      /-
+      by_cases hroot : id = ((eg.uf.union (lookupCanonicalEClassId eg id₁) (lookupCanonicalEClassId eg id₂)).snd)
+      case pos =>
+        simp[UF.union, lookupCanonicalEClassId] at hroot
+        simp[UF.findIdempotent eg.uf hUfc id₁, UF.findIdempotent eg.uf hUfc id₂] at hroot
+        rw[←lookupCanonicalEClassId, ←lookupCanonicalEClassId] at hroot
+        simp[hnq] at hroot
+        simp[hroot] at hlookup
+
+
+
+        sorry
+      case neg =>
+
+        sorry
+      -/
+
+
+
+
+
+/-
+  Yay!
+-/
+
+theorem EGraph.pushPreservesAlwaysInvariants [Analysis α D] (eg : EGraph α D)
+  (h : eg.alwaysInvariants) (en : ENode α) :
+    (push eg en).1.alwaysInvariants := by
+  have hinvar := h
+  unfold EGraph.alwaysInvariants
+  unfold EGraph.alwaysInvariants at h
+  rcases h with ⟨hUfWf, hDv, hAv, hHcEm, hhcv, hepv⟩
+  rcases hUfWf with ⟨hUfv, hUfc, hR, hCmp, hU⟩
   constructor
-  · -- hasRep
-    sorry
-  · -- isComplete
-    sorry
+  · -- wellformed
+    exact eg.pushPreservesWellFormed hinvar en
   constructor
   · -- dirtyValid
-    unfold push
-    dsimp
-    split
-    case h_1 opeid id lookupSome =>
-      exact hDv
-    case h_2 oid lookupNone =>
-      simp only
-      unfold EGraph.dirtyValid
-      intro id hmem
-      dsimp at *
-      unfold UF.isValidID
-      have hmem' := List.mem_cons.mp hmem
-      rcases hmem' with hnew | hold
-      ·
-        simp[hnew, UF.push, UF.size]
-      ·
-        simp[UF.push, UF.size]
-        simp[UF.push, UF.size] at hmem
-        rcases hmem with rfl | hold
-        ·
-          simp
-        ·
-          have hid := hDv id hold
-          simp[UF.isValidID] at hid
-          simp[UF.size] at hid
-          have hpo : id < List.length eg.uf + 1 := Nat.lt_trans hid (Nat.lt_add_one _)
-          exact hpo
+    exact eg.pushPreservesDirty hinvar en
   constructor
   · -- aldrtValid
-    unfold push
-    dsimp only
-    split
-    case h_1 oeid id lookupSome =>
-      exact hAv
-    case h_2 oeid lookupNone =>
-      simp only
-      unfold EGraph.aldrtValid
-      intro id hmem
-      dsimp at *
-      unfold UF.isValidID
-      have hmem' := List.mem_cons.mp hmem
-      rcases hmem' with hnew | hold
-      ·
-        simp[hnew, UF.push, UF.size]
-      ·
-        simp[UF.push, UF.size]
-        simp[UF.push, UF.size] at hmem
-        rcases hmem with rfl | hold
-        ·
-          simp
-        ·
-          have hid := hAv id hold
-          simp[UF.isValidID, UF.size] at hid
-          exact Nat.lt_trans hid (Nat.lt_add_one _)
-  · -- hconsToECMap
+    exact eg.pushPreservesAldrt hinvar en
+  constructor
+  ·
     unfold push
     dsimp only
     split
@@ -116,6 +674,11 @@ theorem pushPreservesAlwaysInvariants [Analysis α D] (eg : EGraph α D)
       simp[hcLookup] at hLookup
 
       sorry
+  constructor-- hconsToECMap
+  ·
+    exact eg.pushPreservesHConsValidity hinvar en
+  · -- ecmapparentsvalid
+    exact eg.pushPreservesECMapParentsValid hinvar en
 
 
 
@@ -144,194 +707,294 @@ theorem pushPreservesAlwaysInvariants'' [Analysis α D] (eg : EGraph α D)
         -- feel like im doing something wrong?
 -/
 
+theorem EGraph.unionPreservesisValid [Analysis α D] (eg : EGraph α D)
+  (h : eg.alwaysInvariants) (id₁ id₂ : EClassId)
+    (h₁ : id₁ < eg.uf.size) (h₂ : id₂ < eg.uf.size) :
+      (union eg id₁ id₂).1.uf.isValid := by
+  unfold EGraph.alwaysInvariants at h
+  rcases h with ⟨hUfwf, hDv, hAv, hHc, hhcv, hecp⟩
+  have hwf := hUfwf
+  rcases hUfwf with ⟨hv, hc, hR, hCmp, hU⟩
+  simp[UF.isValid]
+  intro id cid hmem
+
+  constructor
+  ·
+    simp[UF.isValidID]
+    --have hps := UF.unionPreservesSize eg.uf id₁ id₂
+    dsimp[union] at hmem
+    split at hmem
+    case isTrue aa =>
+      simp at hmem
+      have ⟨hV, hC⟩ := hv id cid hmem
+      simp[union, aa]
+      simp[UF.isValidID] at hV
+      exact hV
+
+    case isFalse bb =>
+      simp at hmem
+      simp[union, bb]
+      have v₁ := UF.findReturnsValid eg.uf hv id₁ h₁
+      have v₂ := UF.findReturnsValid eg.uf hv id₂ h₂
+      have hvs := UF.unionPreservesValid eg.uf hv (lookupCanonicalEClassId eg id₁) (lookupCanonicalEClassId eg id₂) v₁
+      -- have ⟨hl, _⟩ := hvs id cid hmem
+      exact (hvs id cid hmem).1
+  ·
+    simp[UF.isValidID]
+    dsimp[union] at hmem
+    split at hmem
+    case isTrue aa =>
+      simp at hmem
+      have ⟨hV, hC⟩ := hv id cid hmem
+      simp[union, aa]
+      exact hC
+    case isFalse bb =>
+      simp at hmem
+      simp[union, bb]
+      have v₁ := UF.findReturnsValid eg.uf hv id₁ h₁
+      have v₂ := UF.findReturnsValid eg.uf hv id₂ h₂
+      have hvs := UF.unionPreservesValid eg.uf hv (lookupCanonicalEClassId eg id₁) (lookupCanonicalEClassId eg id₂) v₁
+      exact (hvs id cid hmem).2
+
+
+
+
+theorem EGraph.unionPreservesisCanon [Analysis α D] (eg : EGraph α D)
+  (h : eg.alwaysInvariants) (id₁ id₂ : EClassId)
+    (h₁ : id₁ < eg.uf.size) (h₂ : id₂ < eg.uf.size) :
+      (union eg id₁ id₂).1.uf.isCanon := by
+  unfold EGraph.alwaysInvariants at h
+  rcases h with ⟨hUfwf, hDv, hAv, hHc, hhcv, hecp⟩
+  have hwf := hUfwf
+  rcases hUfwf with ⟨hv, hc, hR, hCmp, hU⟩
+  -- isCanon
+  -- have hUPC := UF.unionPreservesCanon eg.uf hc (lookupCanonicalEClassId eg id₁) (lookupCanonicalEClassId eg id₂)
+  dsimp[union]
+  split
+  case isTrue aa =>
+    exact hc
+  case isFalse bb =>
+    simp[lookupCanonicalEClassId] at *
+    exact UF.unionPreservesCanon eg.uf hc (eg.uf.find id₁) (eg.uf.find id₂)
+    -- interesting that the proof got shorter?
+
+    -- simp[UF.union]
+    -- simp[UF.findIdempotent eg.uf hc id₁] at *
+    -- simp[UF.findIdempotent eg.uf hc id₂] at *
+    -- simpa[UF.union, bb] using hUPC
+    -- simp only [bb]
+    --unfold changeLeader
+
+    /-
+    dsimp[UF.union]
+    simp[lookupCanonicalEClassId] at *
+    simp[UF.findIdempotent eg.uf hc, bb]
+    simp [UF.isCanon] at hc
+    -/
+
+theorem EGraph.unionPreservesHasReps [Analysis α D] (eg : EGraph α D)
+  (h : eg.alwaysInvariants) (id₁ id₂ : EClassId)
+    (h₁ : id₁ < eg.uf.size) (h₂ : id₂ < eg.uf.size) :
+      (union eg id₁ id₂).1.uf.hasRep := by
+  unfold EGraph.alwaysInvariants at h
+  rcases h with ⟨hUfwf, hDv, hAv, hHc, hhcv, hecp⟩
+  have hwf := hUfwf
+  rcases hUfwf with ⟨hv, hc, hR, hCmp, hU⟩
+  -- hasRep
+  dsimp[union]
+  split
+  case isTrue aa =>
+    simp[hR]
+  case isFalse bb =>
+    simp only
+    have v₁ := UF.findReturnsValid eg.uf hv id₁ h₁
+    have v₂ := UF.findReturnsValid eg.uf hv id₂ h₂
+    exact UF.unionPreservesReps eg.uf (lookupCanonicalEClassId eg id₁) (lookupCanonicalEClassId eg id₂) hwf v₁ v₂
+
+theorem EGraph.unionPreservesisComplete [Analysis α D] (eg : EGraph α D)
+  (h : eg.alwaysInvariants) (id₁ id₂ : EClassId)
+    (h₁ : id₁ < eg.uf.size) (h₂ : id₂ < eg.uf.size) :
+      (union eg id₁ id₂).1.uf.isComplete := by
+  unfold EGraph.alwaysInvariants at h
+  rcases h with ⟨hUfwf, hDv, hAv, hHc, hhcv, hecp⟩
+  have hwf := hUfwf
+  rcases hUfwf with ⟨hv, hc, hR, hCmp, hU⟩
+  dsimp[union]
+  split
+  case isTrue aa =>
+    simp[hCmp]
+  case isFalse bb =>
+    simp only
+    exact UF.unionPreservesComplete eg.uf (lookupCanonicalEClassId eg id₁) (lookupCanonicalEClassId eg id₂) hwf
+
+theorem EGraph.unionPreservesUniqueKeys [Analysis α D] (eg : EGraph α D)
+  (h : eg.alwaysInvariants) (id₁ id₂ : EClassId)
+    (h₁ : id₁ < eg.uf.size) (h₂ : id₂ < eg.uf.size) :
+      (union eg id₁ id₂).1.uf.uniqueKeys := by
+  unfold EGraph.alwaysInvariants at h
+  rcases h with ⟨hUfwf, hDv, hAv, hHc, hhcv, hecp⟩
+  have hwf := hUfwf
+  rcases hUfwf with ⟨hv, hc, hR, hCmp, hU⟩
+  dsimp[union]
+  split
+  case isTrue aa =>
+    simp[hU]
+  case isFalse bb =>
+    simp only
+    exact UF.unionPreservesUniqueKeys eg.uf hU (lookupCanonicalEClassId eg id₁) (lookupCanonicalEClassId eg id₂)
+
+theorem EGraph.unionPreservesUFWellFormed [Analysis α D] (eg : EGraph α D)
+  (h : eg.alwaysInvariants) (id₁ id₂ : EClassId)
+    (h₁ : id₁ < eg.uf.size) (h₂ : id₂ < eg.uf.size) :
+      (union eg id₁ id₂).1.uf.wellFormed :=
+  ⟨
+    eg.unionPreservesisValid h id₁ id₂ h₁ h₂,
+    eg.unionPreservesisCanon h id₁ id₂ h₁ h₂,
+    eg.unionPreservesHasReps h id₁ id₂ h₁ h₂,
+    eg.unionPreservesisComplete h id₁ id₂ h₁ h₂,
+    eg.unionPreservesUniqueKeys h id₁ id₂ h₁ h₂
+  ⟩
+
+theorem EGraph.unionPreservesDirtyValid [Analysis α D] (eg : EGraph α D)
+  (h : eg.alwaysInvariants) (id₁ id₂ : EClassId)
+    (h₁ : id₁ < eg.uf.size) (h₂ : id₂ < eg.uf.size) :
+      (union eg id₁ id₂).1.dirtyValid := by
+  simp[EGraph.dirtyValid]
+  unfold EGraph.alwaysInvariants at h
+  rcases h with ⟨hUfwf, hDv, hAv, hHc, hhcv, hecp⟩
+  have hwf := hUfwf
+  rcases hUfwf with ⟨hv, hc, hR, hCmp, hU⟩
+  intro id hmem
+  simp[UF.isValidID]
+  unfold union
+  dsimp
+  split
+  case isTrue wasEq =>
+    unfold EGraph.dirtyValid at hDv
+    simp[union, wasEq] at hmem
+    have valid := hDv id hmem
+    simp[UF.isValidID] at *
+    exact valid
+  case isFalse nEq =>
+    --simp[union, nEq] at hmem
+    unfold union at hmem
+    dsimp at hmem
+    simp[nEq] at hmem
+    simp at *
+    have noLength := UF.unionPreservesSize eg.uf (lookupCanonicalEClassId eg id₁) (lookupCanonicalEClassId eg id₂)
+    simp[noLength]
+    rcases hmem with hnew | hold
+    ·
+      simp[hnew]
+      -- have hlv' := UF.unionLeaderValid eg.uf id₁ id₂ h₁ h₂ hv
+      have v₁ := UF.findReturnsValid eg.uf hv id₁ h₁ -- idk what goes in _ actually lol
+      have v₂ := UF.findReturnsValid eg.uf hv id₂ h₂
+      have hlv := UF.unionLeaderValid eg.uf
+        (lookupCanonicalEClassId eg id₁)
+        (lookupCanonicalEClassId eg id₂)
+        v₁ v₂ hv
+      exact hlv
+    ·
+      unfold EGraph.dirtyValid at hDv
+      exact hDv id hold
+
+
+theorem EGraph.unionPreservesAldrtValid [Analysis α D] (eg : EGraph α D)
+  (h : eg.alwaysInvariants) (id₁ id₂ : EClassId)
+    (h₁ : id₁ < eg.uf.size) (h₂ : id₂ < eg.uf.size) :
+      (union eg id₁ id₂).1.aldrtValid := by
+  unfold EGraph.alwaysInvariants at h
+  rcases h with ⟨hUfwf, hDv, hAv, hHc, hhcv, hecp⟩
+  have hwf := hUfwf
+  rcases hUfwf with ⟨hv, hc, hR, hCmp, hU⟩
+  simp[EGraph.aldrtValid]
+  intro id hmem
+  simp[UF.isValidID]
+  unfold union
+  dsimp
+  split
+  case isTrue wasEq =>
+    unfold EGraph.aldrtValid at hAv
+    simp[union, wasEq] at hmem
+    have valid := hAv id hmem
+    simp[UF.isValidID] at *
+    exact valid
+  case isFalse nEq =>
+    unfold union at hmem
+    dsimp at hmem
+    simp[nEq] at hmem
+    simp
+    have noLength := UF.unionPreservesSize eg.uf (lookupCanonicalEClassId eg id₁) (lookupCanonicalEClassId eg id₂)
+    simp[noLength]
+    rcases hmem with hnew | hold
+    ·
+      simp[hnew]
+      have v₁ := UF.findReturnsValid eg.uf hv id₁ h₁
+      have v₂ := UF.findReturnsValid eg.uf hv id₂ h₂
+      exact UF.unionLeaderValid eg.uf
+        (lookupCanonicalEClassId eg id₁) (lookupCanonicalEClassId eg id₂)
+        v₁ v₂ hv
+    ·
+      rcases hold
+      case inr.inl h =>
+        rcases h with ⟨_, b⟩
+        have v₁ := UF.findReturnsValid eg.uf hv id₁ h₁
+        have v₂ := UF.findReturnsValid eg.uf hv id₂ h₂
+        have aaa := UF.unionLeaderValid eg.uf (lookupCanonicalEClassId eg id₁) (lookupCanonicalEClassId eg id₂) v₁ v₂ hv
+        simpa[←b] using aaa -- does simpa help readability
+      case inr.inr h =>
+        -- have aaa := UF.unionPreservesSize eg.uf (lookupCanonicalEClassId eg id₁) (lookupCanonicalEClassId eg id₂)
+        -- simp[aaa] at *
+        simp[EGraph.aldrtValid] at hAv
+        exact hAv id h
+
+theorem EGraph.unionPreservesHConsValidity [Analysis α D] (eg : EGraph α D)
+  (h : eg.alwaysInvariants) (id₁ id₂ : EClassId)
+    (h₁ : id₁ < eg.uf.size) (h₂ : id₂ < eg.uf.size) :
+      (union eg id₁ id₂).1.hconsValidity := by
+  unfold EGraph.alwaysInvariants at h
+  rcases h with ⟨hUfwf, hDv, hAv, hHc, hhcv, hecp⟩
+  have hwf := hUfwf
+  rcases hUfwf with ⟨hv, hc, hR, hCmp, hU⟩
+  simp[EGraph.hconsValidity]
+  intro en id lookupIdSome
+
+  simp[union]
+  split
+  case isTrue h =>
+    simp
+    exact hhcv en id (lookupBeforeUnionSome eg en id₁ id₂ id lookupIdSome)
+  case isFalse h =>
+    simp
+    have bb := hhcv en id (lookupBeforeUnionSome eg en id₁ id₂ id lookupIdSome)
+    have aa := UF.unionPreservesValidID eg.uf (lookupCanonicalEClassId eg id₁)
+                (lookupCanonicalEClassId eg id₂) id bb
+    exact aa
+
+
 theorem unionPreservesAlwaysInvariants [Analysis α D] (eg : EGraph α D)
   (h : eg.alwaysInvariants) (id₁ id₂ : EClassId)
     (h₁ : id₁ < eg.uf.size) (h₂ : id₂ < eg.uf.size) :
       (union eg id₁ id₂).1.alwaysInvariants := by
   unfold EGraph.alwaysInvariants
   unfold EGraph.alwaysInvariants at h
-  rcases h with ⟨hUfwf, hDv, hAv, hHc⟩
+  have hinvar := h
+  rcases h with ⟨hUfwf, hDv, hAv, hHc, hhcv, hecp⟩
   have hwf := hUfwf
   rcases hUfwf with ⟨hv, hc, hR, hCmp, hU⟩
+  constructor
+  exact eg.unionPreservesUFWellFormed hinvar id₁ id₂ h₁ h₂
+  constructor
+  exact eg.unionPreservesDirtyValid hinvar id₁ id₂ h₁ h₂
   repeat constructor
-  · -- isValid
-    simp[UF.isValid]
-    intro id cid hmem
+  exact eg.unionPreservesAldrtValid hinvar id₁ id₂ h₁ h₂
 
-    constructor
-    ·
-      simp[UF.isValidID]
-      --have hps := UF.unionPreservesSize eg.uf id₁ id₂
-      dsimp[union] at hmem
-      split at hmem
-      case isTrue aa =>
-        simp at hmem
-        have ⟨hV, hC⟩ := hv id cid hmem
-        simp[union, aa]
-        simp[UF.isValidID] at hV
-        exact hV
-
-      case isFalse bb =>
-        simp at hmem
-        simp[union, bb]
-        have v₁ := UF.findReturnsValid eg.uf hv id₁ h₁
-        have v₂ := UF.findReturnsValid eg.uf hv id₂ h₂
-        have hvs := UF.unionPreservesValid eg.uf hv (lookupCanonicalEClassId eg id₁) (lookupCanonicalEClassId eg id₂) v₁
-        -- have ⟨hl, _⟩ := hvs id cid hmem
-        exact (hvs id cid hmem).1
-
-    ·
-      simp[UF.isValidID]
-      dsimp[union] at hmem
-      split at hmem
-      case isTrue aa =>
-        simp at hmem
-        have ⟨hV, hC⟩ := hv id cid hmem
-        simp[union, aa]
-        exact hC
-      case isFalse bb =>
-        simp at hmem
-        simp[union, bb]
-        have v₁ := UF.findReturnsValid eg.uf hv id₁ h₁
-        have v₂ := UF.findReturnsValid eg.uf hv id₂ h₂
-        have hvs := UF.unionPreservesValid eg.uf hv (lookupCanonicalEClassId eg id₁) (lookupCanonicalEClassId eg id₂) v₁
-        exact (hvs id cid hmem).2
   constructor
-  · -- isCanon
-    -- have hUPC := UF.unionPreservesCanon eg.uf hc (lookupCanonicalEClassId eg id₁) (lookupCanonicalEClassId eg id₂)
-    dsimp[union]
-    split
-    case isTrue aa =>
-      exact hc
-    case isFalse bb =>
-      simp[lookupCanonicalEClassId] at *
-      exact UF.unionPreservesCanon eg.uf hc (eg.uf.find id₁) (eg.uf.find id₂)
-      -- interesting that the proof got shorter?
-
-      -- simp[UF.union]
-      -- simp[UF.findIdempotent eg.uf hc id₁] at *
-      -- simp[UF.findIdempotent eg.uf hc id₂] at *
-      -- simpa[UF.union, bb] using hUPC
-      -- simp only [bb]
-      --unfold changeLeader
-
-      /-
-      dsimp[UF.union]
-      simp[lookupCanonicalEClassId] at *
-      simp[UF.findIdempotent eg.uf hc, bb]
-      simp [UF.isCanon] at hc
-      -/
-  repeat constructor -- it is obviously possible why did you stop
-  · -- hasRep
-    dsimp[union]
-    split
-    case isTrue aa =>
-      simp[hR]
-    case isFalse bb =>
-      simp only
-      have v₁ := UF.findReturnsValid eg.uf hv id₁ h₁
-      have v₂ := UF.findReturnsValid eg.uf hv id₂ h₂
-      exact UF.unionPreservesReps eg.uf (lookupCanonicalEClassId eg id₁) (lookupCanonicalEClassId eg id₂) hwf v₁ v₂
-  constructor
-  · -- isComplete
-    dsimp[union]
-    split
-    case isTrue aa =>
-      simp[hCmp]
-    case isFalse bb =>
-      simp only
-      exact UF.unionPreservesComplete eg.uf (lookupCanonicalEClassId eg id₁) (lookupCanonicalEClassId eg id₂) hwf
-  · -- uniqueKeys
-    dsimp[union]
-    split
-    case isTrue aa =>
-      simp[hU]
-    case isFalse bb =>
-      simp only
-      exact UF.unionPreservesUniqueKeys eg.uf hU (lookupCanonicalEClassId eg id₁) (lookupCanonicalEClassId eg id₂)
-  constructor
-  · -- dirtyValid
-    simp[EGraph.dirtyValid]
-    intro id hmem
-    simp[UF.isValidID]
-    unfold union
-    dsimp
-    split
-    case isTrue wasEq =>
-      unfold EGraph.dirtyValid at hDv
-      simp[union, wasEq] at hmem
-      have valid := hDv id hmem
-      simp[UF.isValidID] at *
-      exact valid
-    case isFalse nEq =>
-      --simp[union, nEq] at hmem
-      unfold union at hmem
-      dsimp at hmem
-      simp[nEq] at hmem
-      simp at *
-      have noLength := UF.unionPreservesSize eg.uf (lookupCanonicalEClassId eg id₁) (lookupCanonicalEClassId eg id₂)
-      simp[noLength]
-      rcases hmem with hnew | hold
-      ·
-        simp[hnew]
-        -- have hlv' := UF.unionLeaderValid eg.uf id₁ id₂ h₁ h₂ hv
-        have v₁ := UF.findReturnsValid eg.uf hv id₁ h₁ -- idk what goes in _ actually lol
-        have v₂ := UF.findReturnsValid eg.uf hv id₂ h₂
-        have hlv := UF.unionLeaderValid eg.uf
-          (lookupCanonicalEClassId eg id₁)
-          (lookupCanonicalEClassId eg id₂)
-          v₁ v₂ hv
-        exact hlv
-      ·
-        unfold EGraph.dirtyValid at hDv
-        exact hDv id hold
-
-  repeat constructor
-  · -- aldrtValid
-    simp[EGraph.aldrtValid]
-    intro id hmem
-    simp[UF.isValidID]
-    unfold union
-    dsimp
-    split
-    case isTrue wasEq =>
-      unfold EGraph.aldrtValid at hAv
-      simp[union, wasEq] at hmem
-      have valid := hAv id hmem
-      simp[UF.isValidID] at *
-      exact valid
-    case isFalse nEq =>
-      unfold union at hmem
-      dsimp at hmem
-      simp[nEq] at hmem
-      simp
-      have noLength := UF.unionPreservesSize eg.uf (lookupCanonicalEClassId eg id₁) (lookupCanonicalEClassId eg id₂)
-      simp[noLength]
-      rcases hmem with hnew | hold
-      ·
-        simp[hnew]
-        have v₁ := UF.findReturnsValid eg.uf hv id₁ h₁
-        have v₂ := UF.findReturnsValid eg.uf hv id₂ h₂
-        exact UF.unionLeaderValid eg.uf
-          (lookupCanonicalEClassId eg id₁) (lookupCanonicalEClassId eg id₂)
-          v₁ v₂ hv
-      ·
-        rcases hold
-        case inr.inl h =>
-          rcases h with ⟨_, b⟩
-          have v₁ := UF.findReturnsValid eg.uf hv id₁ h₁
-          have v₂ := UF.findReturnsValid eg.uf hv id₂ h₂
-          have aaa := UF.unionLeaderValid eg.uf (lookupCanonicalEClassId eg id₁) (lookupCanonicalEClassId eg id₂) v₁ v₂ hv
-          simpa[←b] using aaa -- does simpa help readability
-        case inr.inr h =>
-          -- have aaa := UF.unionPreservesSize eg.uf (lookupCanonicalEClassId eg id₁) (lookupCanonicalEClassId eg id₂)
-          -- simp[aaa] at *
-          simp[EGraph.aldrtValid] at hAv
-          exact hAv id h
-
-
   · -- hconsToECMap
     sorry
+  constructor
+  exact eg.unionPreservesHConsValidity hinvar id₁ id₂ h₁ h₂
+  exact eg.unionPreservesECMapParentsValid hinvar id₁ id₂
 
 theorem repairPreservesAlwaysInvariants [Analysis α D] (eg : EGraph α D)
   (h : eg.alwaysInvariants) (id : EClassId) :
